registers to stack

w64x4/test/Fp_w64x4.c
@@ -1,22 +1,81 @@
 #include <stdio.h>
 #include <stdint.h>
 #include <assert.h>
-
+#include <string.h>
 
 extern uint64_t* __addm(uint64_t* p, uint64_t* a, uint64_t* b);
+extern uint64_t* __mulm(uint64_t* p, uint64_t* a, uint64_t* b);
+extern uint64_t* __expm(uint64_t* p, uint64_t* a, uint64_t* b);
+
+
+uint64_t tadd[][3][4] =
+ {
+   {  { 0ull , 0ull , 0ull , 0ull }
+    , { 0ull , 0ull , 0ull , 0ull }
+    , { 0ull , 0ull , 0ull , 0ull }
+   }
+ , {  { 1ull , 1ull , 1ull , 1ull }
+    , { 1ull , 1ull , 1ull , 1ull }
+    , { 2ull , 2ull , 2ull , 2ull }
+   }
+ };
+
+
+
+uint64_t tmul[][3][4] =
+ {
+   {  { 0ull , 0ull , 0ull , 0ull }
+    , { 0ull , 0ull , 0ull , 0ull }
+    , { 0ull , 0ull , 0ull , 0ull }
+   }
+ , {  { 1ull , 0ull , 0ull , 0ull }
+    , { 5ull , 5ull , 5ull , 5ull }
+    , { 1ull , 0ull , 0ull , 0ull }
+   }
+
+ };
+
+
+uint64_t texp[][3][4] =
+ {
+   {  { 2ull , 3ull , 0ull , 0ull }
+    , { 2ull , 0ull , 0ull , 0ull }
+    , { 96ull , 0ull , 0ull , 0ull }
+   }
+
+ };
+
+
 
 
 int main() {
-  uint64_t* r;
+  uint64_t result[4]; 
+  int i, b,a;
 
-  uint64_t x[4] = { 5ull, 0ull, 0ull, 0ull };
-  uint64_t y[4] = { 7ull, 0ull, 0ull, 0ull };
-  uint64_t result[4];
- 
-  r = __addm(result, x, y);
+  /* printf("Testing ADDM: "); */
+  /* b = 1; */
+  /* for (i=0; i<2; i++) { */
+  /*  __addm(result, tadd[i][0], tadd[i][1]); */
+  /*  a = memcmp(result, tadd[i][2], sizeof(tadd[i][2])); */
+  /*  b = b && !a; */
+  /* } */
+  /* if (b) printf("OK\n"); else printf("FAIL!\n"); */
 
-  printf("%lu\n", (*result));
-  printf("%lu\n", *(result + (sizeof(unsigned long)/sizeof(uint64_t))));
+
+  __expm(result, texp[0][0], texp[0][1]);
+  printf("%lu\n", *(result+(0*sizeof(uint64_t)/sizeof(uint64_t))));
+
+  
+  /* printf("Testing MULM: "); */
+  /* b = 1; */
+  /* for (i=0; i<2; i++) { */
+  /*  __mulm(result, tmul[i][0], tmul[i][1]); */
+  /*  a = memcmp(result, tmul[i][2], sizeof(tmul[i][2])); */
+  /*  b = b && !a; */
+  /* } */
+  /* if (b) printf("OK\n"); else printf("FAIL!\n"); */
+
+  
 
   return 0;
 }
